---
title: Exponential
---

## Euler constant `e`

$$$
\exp^{x}
$$$

is called the `natural exponential function`

$$$
e=\sum \limits _{n=0}^{\infty }{\frac {1}{n!}}=1+{\frac {1}{1}}+{\frac {1}{1\cdot 2}}+{\frac {1}{1\cdot 2\cdot 3}}+\cdots
$$$
$$$
e= 2.718 281 828...
$$$

## $\exp(ix)$

$$$
\exp^{ix} = cos(x) + i sin(x)
$$$

$$$
\exp^{ix} = \frac{\exp^{ix} + \exp^{-ix}}{2} + i\cdot\frac{\exp^{ix} - \exp^{-ix}}{2i}
$$$

$$$
\exp^{ix} = \frac{\exp^{ix} + \exp^{-ix}}{2} + i\cdot\frac{\exp^{ix} - \exp^{-ix}}{2i}
$$$

$$$
\exp^{ix} = \frac{\exp^{ix} + \exp^{-ix}}{2} + \frac{\exp^{ix} - \exp^{-ix}}{2}
$$$

$$$
\exp^{ix} = \frac{\exp^{ix} + \exp^{-ix} + \exp^{ix} - \exp^{-ix}}{2}
$$$

$$$
\exp^{ix} = \frac{\exp^{ix} + \exp^{ix} + \exp^{-ix} - \exp^{-ix}}{2}
$$$

$$$
\exp^{ix} = \frac{\exp^{ix} + \exp^{ix}}{2}
$$$

$$$
\exp^{ix} = \frac{2\exp^{ix}}{2}
$$$

$$$
\exp^{ix} = \exp^{ix}
$$$

## $\exp(-ix)$

$$$
\exp^{-ix} = cos(x) - i sin(x)
$$$

$$$
\exp^{-ix} = \frac{\exp^{ix} + \exp^{-ix}}{2} - i\cdot\frac{\exp^{ix} - \exp^{-ix}}{2i}
$$$

$$$
\exp^{-ix} = \frac{\exp^{ix} + \exp^{-ix}}{2} - i\cdot\frac{\exp^{ix} - \exp^{-ix}}{2i}
$$$

$$$
\exp^{-ix} = \frac{\exp^{ix} + \exp^{-ix}}{2} - \frac{\exp^{ix} - \exp^{-ix}}{2}
$$$

$$$
\exp^{-ix} = \frac{\exp^{ix} + \exp^{-ix} - (\exp^{ix} - \exp^{-ix})}{2}
$$$

$$$
\exp^{-ix} = \frac{\exp^{ix} + \exp^{-ix} - \exp^{ix} + \exp^{-ix}}{2}
$$$

$$$
\exp^{-ix} = \frac{\exp^{ix} - \exp^{ix} + \exp^{-ix} + \exp^{-ix}}{2}
$$$

$$$
\exp^{-ix} = \frac{\exp^{-ix} + \exp^{-ix}}{2}
$$$

$$$
\exp^{-ix} = \frac{2\exp^{-ix}}{2}
$$$

$$$
\exp^{-ix} = \exp^{-ix}
$$$
